

---

---

[ ]

[ ]

( B )

: \_\_\_\_\_ B \_\_\_\_\_

: 2011 6 24 ( )

4 20

<b>1</b>	<b>2</b>	<b>3</b>	<b>4</b>	<b>5</b>
<b><i>B</i></b>	<b><i>C</i></b>	<b><i>B</i></b>	<b><i>C</i></b>	<b><i>A</i></b>

4 20

1 1/2 2 0 3 1/3 4 0.4772 5 1/4

8

A " " B " "

$P(A|B) = 0.98$   $P(A|\bar{B}) = 0.55$   $P(B) = 0.95$   $P(\bar{B}) = 0.05$  ..... 2

$$P(B|A) = \frac{P(B)P(A|B)}{P(B)P(A|B) + P(\bar{B})P(A|\bar{B})}$$

$$\frac{0.98 \cdot 0.95}{0.98 \cdot 0.95 + 0.55 \cdot 0.05}$$

$$0.97 \quad \frac{1}{2}$$

12

1

$$P\{Y \leq X\} = \int_0^1 \int_x^1 f(x,y) dx dy = \int_0^1 dx \int_0^x (x^2 - \frac{1}{3}xy) dy = \int_0^1 \frac{7}{6} x^3 dx = \frac{7}{24}$$

$\frac{1}{2}$

$$2 \leq x \leq 0 \leq x \leq 1 \quad f_X(x) = 0$$

$$0 \leq x \leq 1 \quad f_X(x) = \int_0^2 (x^2 - \frac{1}{3}xy) dy = 2x^2 - \frac{2}{3}x$$

$$X \quad f_X(x) = \begin{cases} 2x^2 - \frac{2}{3}x, & 0 \leq x \leq 1 \\ 0, & \text{otherwise} \end{cases}$$

1/2 6

10

$$Z = X + Y$$

$$F_Z(z) = P\{Z \leq z\} = P\{X + Y \leq z\} = \int_{x+y \leq z} f(x,y) dx dy$$

$$\int_{x+y \leq z} f_X(x)f_Y(y) dx dy$$

$$(1) z \leq 0 \quad F_Z(z) = 0$$

$$2 \leq z \leq 1 \quad F_Z(z) = \int_{x+y \leq z} f_X(x)f_Y(y) dx dy = \int_0^z dx \int_0^{z-x} e^{-y} dy$$

$$\int_0^z e^{-y} dy \Big|_0^{z-x} dx = \int_0^z [1 - e^{-(x+z)}] dx = [x - e^{-(x+z)}]_0^z = z - 1 + e^{-z}$$

$$3 \leq z \leq 1 \quad F_Z(z) = \int_{x+y \leq z} f_X(x)f_Y(y) dx dy = \int_0^1 dx \int_0^{z-x} e^{-y} dy$$

$$\int_0^1 [1 - e^{-(x+z)}] dx = [x - e^{-(x+z)}]_0^1 = 1 - e^{-(1+z)} - e^{-z} = 1 - e^{-z}(1 + e)$$

$$Z = X + Y$$

$$0, \quad z \leq 0$$

$$F_Z(z) = \begin{cases} z - 1 + e^{-z}, & 0 \leq z \leq 1 \\ 1 - e^{-z}(1 + e), & z \geq 1 \end{cases} \quad 1/2$$

8

$$Z = X + Y$$

$$f_Z(x) = \frac{dF_Z(z)}{dz} = \begin{cases} 0, & z \leq 0 \\ 1 - e^{-z}, & 0 \leq z \leq 1 \\ e^{-z}(e - 1), & z \geq 1 \end{cases}$$

1/2 2

10

$$X \sim B(10000, 0.8)$$

$$X \sim B(10000, 0.8)$$

$$EX = 10000 \cdot 0.8 = 8000 \quad DX = 10000 \cdot 0.8 \cdot 0.2 = 1600$$

1/2 4

$$P\{7920 \leq X \leq 8080\} = P\left\{\frac{7920 - 8000}{\sqrt{1600}} \leq \frac{X - 8000}{\sqrt{1600}} \leq \frac{8080 - 8000}{\sqrt{1600}}\right\}$$

$$P\left\{-2 \leq \frac{X - 8000}{\sqrt{1600}} \leq 2\right\} \quad (2) \quad (2)$$

$$2 \cdot (2) - 1 = 2 \cdot 0.9772 - 1 = 0.9544$$

1/2 6

10

$$(U, V) \quad (1, 1), (1, 2), (2, 1), (2, 2)$$

$$P\{U = 1, V = 1\} = P\{X = 1, Y = 1\} = P\{X = 1\}P\{Y = 1\} = \frac{1}{9}$$

$$P\{U = 2, V = 2\} = P\{X = 2, Y = 2\} = P\{X = 2\}P\{Y = 2\} = \frac{4}{9}$$

$$P\{U = 1, V = 2\} = 0$$

$$P\{U = 2, V = 1\} = 1 - \frac{1}{9} - \frac{4}{9} = \frac{4}{9}$$

$$(X, Y)$$

		$U$	
		1	2
$V$	1	1/9	4/9
	2	0	4/9

1/2 6

$$L(\boldsymbol{\theta}) = \prod_{i=1}^n P(X_i = x_i) = \prod_{i=1}^n \frac{e^{-\theta} \theta^{x_i}}{x_i!} = e^{-n\theta} \prod_{i=1}^n \frac{\theta^{x_i}}{x_i!}$$

$$\ln L(\boldsymbol{\theta}) = \left( \sum_{i=1}^n x_i \right) \ln \theta - n\theta - \sum_{i=1}^n \ln x_i!$$

$$\frac{d \ln L(\boldsymbol{\theta})}{d\theta} = \frac{\sum_{i=1}^n x_i}{\theta} - n,$$

$$\frac{d \ln L(\boldsymbol{\theta})}{d\theta} = 0,$$

$$\hat{\theta} = \frac{1}{n} \sum_{i=1}^n x_i$$